


Reference 

[[Cartesian Product]]

1.2.2 Principle of Mathematical Induction prove:

Proof: Suppose to the contrary that $S\neq N$ 

Since N\s
$m\in IN,m\notin S$  

Since $m\in N,m-1\in N$

Then $m-1<m$

$m-1\notin N/S$

$m-1$


2. For every $k\geq n_0$ , if $P(k)$ is true, then $P(k+1)$ is true

Since $k\geq n_0$, $k-n_0+1\in S$ , $k+1-n_0\in S$, $(k-n_0+1)\in S$

If we replace  $k-n_0+1$ by $m$, we find $m\in N$ is arbitray and satisfy,

$m\in S => m+1\in S$ 

$S=\{n\in N: P(n) \ is\ true\}$ 
